lib/Lib.ByteSequence.fsti
@@ -103,6 +103,18 @@ inline_for_extraction
 val uints_from_bytes_be: #t:inttype{~(t == U1)} -> #l:secrecy_level -> #len:size_nat{len * numbytes t < pow2 32}
   -> lbytes_l l (len * numbytes t) -> lseq (uint_t t l) len
 
+inline_for_extraction
+val uint_at_index_le: #t:inttype{~(t == U1)} -> #l:secrecy_level -> #len:size_nat{len * numbytes t < pow2 32}
+  -> b:lbytes_l l (len * numbytes t) 
+  -> idx:nat{idx < len}
+  -> u:uint_t t l{u == (uints_from_bytes_le #t #l #len b).[idx]}
+
+inline_for_extraction
+val uint_at_index_be: #t:inttype{~(t == U1)} -> #l:secrecy_level -> #len:size_nat{len * numbytes t < pow2 32}
+  -> b:lbytes_l l (len * numbytes t) 
+  -> idx:nat{idx < len}
+  -> u:uint_t t l{u == (uints_from_bytes_be #t #l #len b).[idx]}
+
 val nat_from_intseq_le_slice_lemma: #t:inttype -> #l:secrecy_level -> #len:size_nat
   -> b:lseq (uint_t t l) len -> i:nat{i <= len} ->
   Lemma (nat_from_intseq_le b == nat_from_intseq_le (Seq.slice b 0 i) + pow2 (i * bits t) * nat_from_intseq_le (Seq.slice b i len))
